Working on Type/Value substitution for SystemF

proof/SystemF/Context.v
@@ -28,8 +28,15 @@ Definition extend {A:Type} (rest:partial_map A) (x:name) (T:A)
 Hint Unfold extend.
 
 
-(* An extended contexted contains the member we extended it with. 
- *)
+Definition map {A B:Type} (f : A -> B) (ctx:partial_map A)
+ := fun x 
+ => match ctx x with
+     | none    => none
+     | some T  => some (f T)
+    end.
+
+
+(* An extended contexted contains the member we extended it with. *)
 Lemma extend_eq 
  : forall A (ctx: partial_map A) x T
  , (extend ctx x T) x = some T.
@@ -37,13 +44,11 @@ Proof.
  intros. unfold extend.  
  rewrite <- beq_name_refl. auto.
 Qed.
-
 Hint Resolve extend_eq.
 
 
 (* We can skip over elements in a context that don't match 
-   then one we're looking for.
- *)
+   then one we're looking for. *)
 Lemma extend_neq
  :  forall A (ctx: partial_map A) x1 T x2
  ,  x2 <> x1
@@ -53,13 +58,24 @@ Proof.
  remember (beq_name x2 x1) as e. destruct e.
  apply true_name_eq in Heqe. subst. contradict H. auto. auto.
 Qed.
-
 Hint Resolve extend_neq.
 
 
+Lemma extend_pack
+ :  forall A (ctx: partial_map A) x1 T1 T2 
+ ,  extend (extend ctx x1 T1) x1 T2
+ =  extend ctx x1 T2.
+Proof.
+ intros.
+ apply functional_extensionality. intro.
+ unfold extend.
+ remember (beq_name x1 x) as e. destruct e; auto.
+Qed.
+Hint Resolve extend_pack.
+
+
 (* If two elements in a context are bound to different names, 
-   then we can swap their order. 
- *)
+   then we can swap their order. *)
 Lemma extend_swap
  :   forall A (ctx: partial_map A) x T1 y T2
  ,   x <> y
@@ -75,5 +91,4 @@ Proof.
   apply true_name_eq in Heqe2. subst. contradict H. trivial.
   trivial. trivial.
 Qed.
- 
 Hint Resolve extend_swap.
