proof/SystemF/SubTypeValue.v
@@ -1,18 +1,77 @@
 
 Require Import KiJudge.
 Require Import TyJudge.
+Require Import Program.
+
+Definition substTTE a T2 tenv
+ := map (substTT a T2) tenv.
 
 (* Substitution of types in values preserves typing.
  *)
 Lemma subst_type_value
- :  forall kenv tenv a t1 t2 T1 T2 K2
- ,  (forall z, freeX z t2 -> freshX z t1)
+ :  forall kenv tenv a t1 T1 T2 K2
+ ,  (forall z, freeT z T2 -> freshX z t1)
  -> TYPE (extend kenv a K2) tenv  t1  T1
  -> KIND      kenv                T2  K2
- -> TYPE kenv tenv  (substTX a T2 t1) T1.  (* TODO, sub into tyenv *)
+ -> TYPE kenv
+         (substTTE a T2 tenv)
+         (substTX  a T2 t1)
+         (substTT  a T2 T1).  
 Proof.
- intros kenv tenv a t1 t2 T1 T2 K2.
+ intros kenv tenv a t1 T1 T2 K2.
  generalize dependent kenv.
  generalize dependent tenv.
  generalize dependent T1.
- induction t1.
+ induction t1; intros; inversions H0.
+
+ Case "XVar".
+  apply TYVar; auto.
+  unfold substTTE. unfold map. remember (tenv n) as e. destruct e.
+   inversions H6. inversions H6. auto.
+
+ Case "XLam". simpl.
+  eapply TYLam. auto.
+  eapply type_tyenv_invariance.
+   apply IHt1; eauto.
+    intros. apply H in H0. inversions H0. auto.
+    eauto.
+    intros. unfold extend. remember (beq_name n x) as e. destruct e.
+     apply true_name_eq in Heqe. subst.
+      unfold substTTE. unfold map.
+      rewrite <- beq_name_refl. auto.
+     apply false_name_neq in Heqe.
+      unfold substTTE. unfold map.
+      rewrite <- neq_name_false. auto. auto. 
+
+ Case "XApp". simpl.
+  eapply TYApp.
+   eapply IHt1_1 in H6. eauto.
+    intros. apply H in H0. inversions H0. auto. auto. fold substTT.
+   eapply IHt1_2 in H8. eauto.
+    intros. apply H in H0. inversions H0. auto. auto.
+
+ Case "XLAM". simpl.
+  remember (beq_name a n) as e. destruct e.
+  apply true_name_eq in Heqe. subst.
+   rewrite -> extend_pack in H8.
+   rewrite -> extend_swap in H8.
+
+  apply TYLAM. auto.
+   apply IHt1 in H8.
+
+
+eauto.
+  apply true_name_eq in Heqe. subst.
+   eapply type_tyenv_invariance in H8. eauto.
+   eauto.
+   intros. unfold substTTE. unfold map. 
+   apply equal_f.
+
+unfold substTT.
+   intros.
+  eapply IHt1 in H1.
+   eauto.
+
+
+
+
