proof/SystemF/Progress.v
@@ -29,32 +29,29 @@ Proof.
   SCase "t1 value".
    destruct IHHt2; auto.
    SSCase "t2 value".
-    inversion H. subst.
-    exists (substXX x t2 t). 
-     apply EVAppLam. auto.
-    subst. inversion Ht1.
+    inversions H.
+     exists (substXX x t2 t). apply EVAppLam. auto.
+     inversion Ht1.
    SSCase "t2 steps".
     destruct H0 as [t2' Htsp].
-    inversion H. subst.
-    exists (XApp (XLam x T t) t2').
-     apply EVApp2; auto.
-    subst. inversion Ht1.
+    inversions H.
+     exists (XApp (XLam x T t) t2'). apply EVApp2; auto.
+     inversion Ht1.
   SCase "t1 steps".
    destruct H as [t1' Htsp].
-   exists (XApp t1' t2).
-   apply EVApp1. auto.
+   exists (XApp t1' t2). apply EVApp1. auto.
 
  Case "XLAM".
-   left. apply Value_LAM.
-   apply TYLAM in Ht.
+   left.
+   apply Value_LAM. apply TYLAM in Ht.
    eapply check_empty_is_closed. subst. eauto. auto.
 
  Case "XAPP".
    right.
    destruct IHHt; auto.
    SCase "t1 value".
-    inversion H0. subst.
-    inversion Ht. eauto.
+    inversions H0.
+    inversion  Ht. eauto.
    SCase "t1 steps".
     destruct H0 as [t1' Hstp].
     exists (XAPP t1' T2).
